platform/Depl/Depl.v
@@ -22,29 +22,14 @@ Bind Scope pred_scope with pred.
 Infix "*" := Star : pred_scope.
 Notation "'EX' x , p" := (Exists x p%pred) (at level 89) : pred_scope.
 Notation "'Emp'" := (Pure (fun _ => True)) : pred_scope.
-
-
-
-(** * Program expression notations *)
-
-Require Import Depl.Statements.
-
-Definition Var'' : string -> expr := Var.
-Coercion Var'' : string >-> expr.
-Coercion Const : W >-> expr.
-
-
-(** * Program statement notations *)
-
-Infix "<-" := Assign : stmt_scope.
-Infix ";;" := Seq : stmt_scope.
-Notation "'Return' e" := (Ret e) : stmt_scope.
-
-Delimit Scope stmt_scope with stmt.
-Bind Scope stmt_scope with stmt.
+Notation "e1 = e2" := (Equal e1%expr e2%expr) : pred_scope.
+Notation "# X ( e1 , .. , eN )" := (Named X (@cons expr e1%expr (.. (@cons expr eN%expr nil) ..)))
+  (X at level 0) : pred_scope.
 
 
 (** * Program function spec notations *)
+
+Require Import Depl.Statements.
 
 Record fspec := {
   SpecVars_ : list fo_var;
@@ -77,7 +62,28 @@ Delimit Scope spec_scope with spec.
 Bind Scope spec_scope with fspec.
 
 
+(** * Program expression notations *)
+
+Definition Var'' : string -> expr := Var.
+Coercion Var'' : string >-> expr.
+Coercion Const : W >-> expr.
+
+
+(** * Program statement notations *)
+
+Infix "<-" := Assign : stmt_scope.
+Infix ";;" := Seq : stmt_scope.
+Notation "'Return' e" := (Ret e) : stmt_scope.
+Notation "x <-- # con ( e1 , .. , eN )" := (Allocate x con (@cons expr e1 (.. (@cons expr eN nil) ..)))
+  (no associativity, at level 95, con at level 0) : stmt_scope.
+
+Delimit Scope stmt_scope with stmt.
+Bind Scope stmt_scope with stmt.
+
+
 (** * Program function notations *)
+
+Require Import Depl.AlgebraicDatatypes.
 
 Record func := {
   Name_ : string;
@@ -86,24 +92,72 @@ Record func := {
   Body_ : stmt
 }.
 
-Notation "'dfunction' name [ p ] b 'end'" := {|
+Inductive defn :=
+  | Dtype (dt : datatype)
+  | Func (fu : func).
+
+Notation "'dfunction' name [ p ] b 'end'" := (Func {|
   Name_ := name;
   Spec_ := p%spec;
   Locals_ := nil;
   Body_ := b%stmt
-|} (no associativity, at level 95, name at level 0, only parsing) : func_scope.
+|}) (no associativity, at level 95, name at level 0, only parsing) : func_scope.
 
-Notation "'dfunction' name [ p ] 'Locals' x1 , .. , xN 'in' b 'end'" := {|
+Notation "'dfunction' name [ p ] 'Locals' x1 , .. , xN 'in' b 'end'" := (Func {|
   Name_ := name;
   Spec_ := p%spec;
   Locals_ := cons x1 (.. (cons xN nil) ..);
   Body_ := b%stmt
-|} (no associativity, at level 95, name at level 0, only parsing) : func_scope.
+|}) (no associativity, at level 95, name at level 0, only parsing) : func_scope.
 
 Delimit Scope func_scope with func.
 
 
+(** * Datatype definition notations *)
+
+Notation "# con ( nr1 , .. , nrN ; r1 , .. , rN ) p" := {|
+  Name := con;
+  Recursive := cons r1 (.. (cons rN nil) ..);
+  Nonrecursive := cons nr1 (.. (cons nrN nil) ..);
+  Condition := p%pred
+|} (no associativity, at level 95, con at level 0) : con_scope.
+
+Notation "# con ( ; r1 , .. , rN ) p" := {|
+  Name := con;
+  Recursive := cons r1 (.. (cons rN nil) ..);
+  Nonrecursive := nil;
+  Condition := p%pred
+|} (no associativity, at level 95, con at level 0) : con_scope.
+
+Notation "# con ( nr1 , .. , nrN ; ) p" := {|
+  Name := con;
+  Recursive := nil;
+  Nonrecursive := cons nr1 (.. (cons nrN nil) ..);
+  Condition := p%pred
+|} (no associativity, at level 95, con at level 0) : con_scope.
+
+Delimit Scope con_scope with con.
+Bind Scope con_scope with con.
+
+Notation "{{ x 'with' .. 'with' y }}" := (cons x%con .. (cons y%con nil) ..) (only parsing) : cons_scope.
+Delimit Scope cons_scope with cons.
+
+Notation "'dtype' name = cs" := (Dtype (name, cs%cons))
+  (no associativity, at level 95, name at level 0, cs at level 0) : func_scope.
+
+
 (** * Program module notations *)
+
+Fixpoint separate (ds : list defn) : list datatype * list func :=
+  match ds with
+    | nil => (nil, nil)
+    | Dtype dt :: ds =>
+      let (dts, fs) := separate ds in
+        (dt :: dts, fs)
+    | Func fu :: ds =>
+      let (dts, fs) := separate ds in
+        (dts, fu :: fs)
+  end.
 
 Require Import Depl.CompileModule.
 
@@ -120,8 +174,9 @@ Definition funcOut (f : func) : function := {|
 Notation "{{ x 'with' .. 'with' y }}" := (cons x%func .. (cons y%func nil) ..) (only parsing) : funcs_scope.
 Delimit Scope funcs_scope with funcs.
 
-Notation "'dmodule' name fs" := (compileModule nil {| MName := name;
-  Functions := map funcOut fs%funcs |})
+Notation "'dmodule' name ds" := (let (dts, fs) := separate ds%funcs in
+                                 compileModule dts {| MName := name;
+                                                      Functions := map funcOut fs |})
   (no associativity, at level 95, name at level 0, only parsing).
 
 
@@ -130,20 +185,49 @@ Notation "'dmodule' name fs" := (compileModule nil {| MName := name;
 (* There is a somewhat intricate little dance here to get good reduction behavior.
  * First, we normalize enough to expose potentially worrying uses of [in_dec string_dec],
  * where delta-expanding those identifiers would lead to unpleasantly large terms. *)
-Ltac depl_cbv1 := cbv beta iota zeta delta [CompileModule.makeVcs CompileModule.Functions map funcOut
-  CompileModule.functionVc CompileModule.Postcondition CompileModule.Formals
-  SpecVars_ Formals_ Precondition_ Postcondition_
-  Name_ Spec_ Locals_ Body_ Logic.wellScoped CompileModule.Body app
-  CompileModule.Locals CompileModule.Precondition CompileModule.SpecVars
-  Logic.normalize Statements.stmtD Statements.exprD Statements.sentail Cancel.cancel
-  Cancel.findMatchings Logic.NQuants Logic.NImpure Logic.NPure Logic.nsubst].
+Ltac depl_cbv1 := cbv beta iota zeta
+   delta [CompileModule.makeVcs CompileModule.Functions map funcOut
+         CompileModule.functionVc CompileModule.Postcondition
+         CompileModule.Formals SpecVars_ Formals_ Precondition_
+         Postcondition_ Name_ Spec_ Locals_ Body_ Logic.wellScoped
+         CompileModule.Body app CompileModule.Locals
+         CompileModule.Precondition CompileModule.SpecVars Logic.normalize
+         Statements.stmtD Statements.exprD Statements.sentail Cancel.cancel
+         Cancel.findMatchings Logic.NQuants Logic.NImpure Logic.NPure
+         Logic.nsubst Statements.lookupCon Statements.lookupCon'
+         AlgebraicDatatypes.normalizeDatatype fst snd
+         AlgebraicDatatypes.NName AlgebraicDatatypes.normalizeCon
+         AlgebraicDatatypes.Name AlgebraicDatatypes.Nonrecursive
+         AlgebraicDatatypes.Recursive AlgebraicDatatypes.Condition
+         AlgebraicDatatypes.NRecursive AlgebraicDatatypes.NNonrecursive
+         AlgebraicDatatypes.NCondition plus sumbool_rec sumbool_rect
+         Logic.notsInList Logic.notInList string_rec string_rect
+         append Ascii.ascii_dec Ascii.ascii_rec Ascii.ascii_rect
+         Bool.bool_dec bool_rec bool_rect eq_rec_r eq_rec eq_rect eq_sym
+         Statements.exprsD
+         AlgebraicDatatypes.allocatePre AlgebraicDatatypes.nsubsts
+         Peano_dec.eq_nat_dec string_eq ascii_eq Bool.eqb andb nat_rec nat_rect length
+         AlgebraicDatatypes.recursives Cancel.findMatching Logic.psubst
+         Logic.esubst Var' Cancel.sub_expr Cancel.findMatching'
+         Cancel.unify_pred Cancel.unify_expr Cancel.fos_set Cancel.unify_args Var''
+         Statements.vars_set].
+
+(** Now we [destruct] string comparisons. *)
+Ltac streq :=
+  repeat match goal with
+           | [ |- context[string_dec ?X ?Y] ] =>
+             destruct (string_dec X Y); try congruence; [ clear ]
+           | [ |- context[in_dec string_dec ?X ?Y] ] =>
+             destruct (in_dec string_dec X Y);
+               try (exfalso; simpl in *; intuition congruence); [ clear ]
+         end.
 
 (* Next, we find the little marker predicates we used in Cancel to indicate where the
  * troubling [in_dec]s are, and we hide them inside this guy here. *)
 Definition sin_dec := in_dec string_dec.
 Ltac switch_to_sin_dec :=
   repeat match goal with
-           | [ |- context[Cancel.hide_sub ?s] ] =>
+           | [ |- appcontext[Cancel.hide_sub ?s] ] =>
              let s' := fresh "s'" in pose (s' := s);
                change (in_dec string_dec) with sin_dec in s';
                  let s'' := eval unfold s' in s' in
@@ -165,10 +249,12 @@ Ltac depl_cbv2 := cbv beta iota zeta delta [CompileModule.makeVcs CompileModule.
   in_dec list_rec list_rect
   string_dec string_rec string_rect
   Ascii.ascii_dec Ascii.ascii_rec Ascii.ascii_rect sumbool_rec sumbool_rect
-  Bool.bool_dec bool_rec bool_rect eq_rec_r eq_rec eq_rect eq_sym append].
+  Bool.bool_dec bool_rec bool_rect eq_rec_r eq_rec eq_rect eq_sym append
+  allocatePre nsubsts recursives
+  lookupCon lookupCon' normalizeDatatype fst snd].
 
 (* Put them all together. *)
-Ltac depl_cbv := depl_cbv1; switch_to_sin_dec; depl_cbv2.
+Ltac depl_cbv := depl_cbv1; streq; switch_to_sin_dec.
 
 Ltac isConst E :=
   match E with
@@ -182,6 +268,13 @@ Ltac isConst E :=
 (* Simplify one of the syntactic well-formedness side conditions generated by [compileModule_ok]. *)
 Ltac depl_wf :=
   match goal with
+    | [ |- stmtV _ _ _ ] => simpl; tauto
+    | [ |- Compile.datatypesWf _ ] =>
+      repeat (econstructor; simpl in *; intros); simpl in *; intuition (try congruence);
+        match goal with
+          | [ H : forall x : Logic.fo_var, _ -> _ = _ |- _ ] =>
+            repeat rewrite H by tauto; reflexivity
+        end
     | [ |- forall fE fE' : Logic.fo_var -> Logic.dyn, (forall x, In x _ -> fE x = fE' x) -> _ = _ ] =>
       simpl; intros fE fE' Heq;
         repeat rewrite Heq by tauto; reflexivity
@@ -196,12 +289,20 @@ Ltac depl_wf :=
     | [ |- In ?x ?ls ] => isConst x; isConst ls; simpl; tauto
     | [ |- forall x : Logic.fo_var, In x _ -> exists e : Logic.expr, _ ] =>
       simpl; intuition (subst; simpl; eauto)
-  end.
+    | [ |- forall fE fE' : Logic.fo_var -> Logic.dyn, _ -> forall e : Logic.expr, In _ _ -> _ ] =>
+      simpl; intuition (subst; auto)
+  end;
+  try match goal with
+        | [ |- Logic.exprD _ _ = Logic.exprD _ _ ] =>
+          simpl; match goal with
+                   | [ H : forall x : Logic.fo_var, _ |- _ ] => repeat rewrite H by tauto
+                 end; reflexivity
+      end.
 
 Ltac depl := apply CompileModule.compileModule_ok; [ constructor
   | hnf; NoDup
   | reflexivity
-  | constructor
+  | depl_wf
   | reflexivity
   | depl_cbv;
     match goal with
@@ -209,5 +310,5 @@ Ltac depl := apply CompileModule.compileModule_ok; [ constructor
     end;
     repeat match goal with
              | [ |- _ /\ _ ] => split
-           end; try depl_wf
+           end; repeat depl_wf
   | simpl; discriminate ].
