platform/Depl/examples/Basic.v
@@ -1,0 +1,44 @@
+(** * Basic examples that define datatypes *)
+
+Require Import Depl.
+
+
+(** * The simplest example that defines (but does not use!) a datatype *)
+
+Definition unused := dmodule "m" {{
+  dtype "unit" = {{ #"tt"("dummy";) "this" = |^_, !tt| }}
+  with dfunction "f" [
+    ARGS()
+    PRE Emp
+    POST Emp
+  ]
+    Return 0
+  end
+}}.
+
+Theorem unusedOk : moduleOk unused.
+Proof.
+  depl; auto.
+Qed.
+
+
+(** * Now, let's actually construct a value! *)
+
+Definition unit := dmodule "m" {{
+  dtype "unit" = {{ #"tt"("dummy";) "this" = |^_, !tt| }}
+  with dfunction "f" [
+    ARGS()
+    PRE Emp
+    POST #"unit"(|^_, !tt|, "result")
+  ]
+    Locals "ret" in
+    "ret" <-- #"tt"(0);;
+    Return "ret"
+  end
+}}.
+
+Theorem unitOk : moduleOk unit.
+Proof.
+  depl; auto.
+  admit. (* Cancelation not matching free variables properly. :-( *)
+Qed.
